Hs/Translator/Types.lean
@@ -3,60 +3,6 @@ import Hs.Translator.Kinds
 set_option linter.unusedVariables false
 
 @[simp]
-def compile_type_meh (Γ : Ctx Term) : Term -> HsTerm -> DsM Term
-  -- A → B
-  | ★ , .HsBind2 .arrow A B => do
-  let A' <- compile_type_meh Γ ★ A
-  let B' <- compile_type_meh (.empty :: Γ) ★ B
-  .ok (.bind2 .arrow A' B')
-
-  -- A ⇒ B
-  | ★ , .HsBind2 .farrow A B => do
-  let A' <- compile_type_meh Γ ★ A
-  let B' <- compile_type_meh (.empty :: Γ) ★ B
-  .ok (.bind2 .arrow A' B')
-
-  -- ∀[A] B
-  | ★ , .HsBind2 .all A B => do
-  let A' <- compile_kind Γ □ A
-  let B' <- compile_type_meh (.kind A' :: Γ) ★ B
-  .ok (.bind2 .all A' B')
-
-  -- A ⬝ B ⬝ D .. (List α etc.)
-  | exp_κ, τ => do
-    match tnfp : τ.neutral_form with
-    | .none => .error ("compile_type_meh neutral form" ++ repr τ)
-    -- A [B, C, ..]
-    | .some (h, sp) =>
-      match h with
-      | `#h =>
-        let τ <- .toDsM ("compile_type_meh get type" ++ Std.Format.line ++ repr Γ ++ Std.Format.line ++ repr h)
-              ((Γ d@ h).get_type)
-
-        -- split the head kind arrow
-        -- A : k1 -> k2 -> ... -> k_ret
-        let (κs, actual_κ) <- .toDsMq (Term.split_kind_arrow τ)
-
-        -- make sure the lengths match up
-        if exp_κ == actual_κ && sp.all (λ x => x.1 == .kind) && κs.length == sp.length
-        then
-          -- compile each type with the expected kind
-          -- [(B : k1), (C : K2) ...]
-          let args' <- (κs.zip sp).mapM
-                    (λ arg =>
-                      compile_type_meh Γ arg.1 (arg.2.2))
-          .ok (Term.mk_kind_app h args')
-        else .error ("compile_type_meh ill kinded" ++ repr τ)
-      | _ => .error ("compile_type_meh head" ++ repr h ++ repr sp)
-termination_by _ t => t.size
-decreasing_by (
-any_goals (simp; omega)
-· sorry -- where does arg come from? :(
-)
-
-
-
-@[simp]
 def compile_type (Γ : Ctx Term) : Term -> HsTerm -> DsM Term
   | ★ , .HsBind2 .arrow A B => do
   let A' <- compile_type Γ ★ A
@@ -84,15 +30,13 @@ def compile_type (Γ : Ctx Term) : Term -> HsTerm -> DsM Term
         match spk : Term.split_kind_arrow k with
         | .none => .error ("no split arrow kind" ++ repr k)
         | .some (κs, actual_κ) => do
-          have lem : Term.mk_kind_arrow actual_κ κs = k := by
-            sorry
           if exp_κ == actual_κ && sp.all (λ x => x.1 == .kind) && κs.length == sp.length
           then
             let zz := List.attach (List.zip (List.attach κs) (List.attach sp))
             let args' <- zz.mapM
                       (λ arg =>
                         compile_type Γ arg.val.1 (arg.val.2.val.2))
-            .ok (Term.mk_kind_app h args')
+            .ok (Term.mk_kind_app_rev #h args'.reverse)
           else .error ("compile_type ill kinded" ++ repr τ)
       | _ => .error ("compile_type head" ++ repr h ++ repr sp)
 termination_by _ t => t.size
